Больше лемм богу лемм!

Test.Float.fsti
@@ -2,6 +2,7 @@ module Test.Float
 
 open FStar.Printf
 open FStar.Mul
+module Lemmas = FStar.Math.Lemmas
 
 new val float : eqtype
 
@@ -16,51 +17,88 @@ let float_extension : extension_parser = fun s ->
 type mant_pow' = int & int
 type mant_pow = x: mant_pow'{x._1 % 10 = 0 ==> (x._1 = 0 /\ x._2 = 0)}
 
+private let ( +> ) (mp: mant_pow') (n: int) = (fst mp, snd mp + n)
+private let ( *< ) (mp: mant_pow') (n: int) = (fst mp * n, snd mp)
+private let ( /< ) (mp: mant_pow') (n: nonzero) = (fst mp / n, snd mp)
+private let ( >=< ) (a b: int) =
+  a > 0 && b > 0 ||
+  a = 0 && b = 0 ||
+  a < 0 && b < 0
+
+let lemma_mant_mul (mp: mant_pow') (a b: int) : Lemma (mp *< a *< b = mp *< (a * b)) = ()
+
+
 let rec pow10 (x: nat) : GTot pos =
   match x with
   | 0 -> 1
   | _ -> 10 * pow10 (x - 1)
-let rec norm_pair (mp: mant_pow') : Tot mant_pow (decreases abs (fst mp)) =
-  let mantissa = fst mp in
-  let power = snd mp in
-  if mantissa = 0
-  then 0, 0
-  else if mantissa % 10 = 0
-       then norm_pair (mantissa / 10, power + 1)
-       else mp
+let rec norm_pair (mp': mant_pow') : Pure mant_pow
+  (requires True)
+  (ensures fun mp ->
+    (fst mp' >=< fst mp) /\
+    (fst mp' <> 0 ==>
+      snd mp' <= snd mp /\
+      fst mp' = fst mp * pow10 (snd mp - snd mp') /\
+      fst mp = fst mp' / pow10 (snd mp - snd mp')))
+  (decreases abs (fst mp'))
+  =
+  let mantissa = fst mp' in
+  let power = snd mp' in
+  match mantissa, mantissa % 10 with
+  | 0, _ -> 0, 0
+  | _, 0 -> 
+    let mp = norm_pair (mantissa / 10, power + 1) in
+    Lemmas.cancel_mul_div (fst mp) (pow10 (snd mp - snd mp'));
+    mp
+  | _, _ -> mp'
 
-let rec lemma_norm_pow_add (n: int) (mp': mant_pow') (mp_': mant_pow') : Lemma 
-  (requires fst mp' <> 0 /\ mp_' = (fst mp', snd mp' + n))
-  (ensures (let mp = norm_pair mp' in norm_pair mp_' = (fst mp, snd mp + n)))
+let rec lemma_norm_pow_inj (n: int) (mp': mant_pow') : Lemma
+  (requires fst mp' <> 0)
+  (ensures norm_pair (mp' +> n) = norm_pair mp' +> n)
   (decreases abs (fst mp'))
   =
   match fst mp' % 10 with
-  | 0 -> 
-    let mp'' = (fst mp' / 10, snd mp' + 1) in
-    let mp_'' = (fst mp_' / 10, snd mp_' + 1) in
-    lemma_norm_pow_add n mp'' mp_''
+  | 0 -> lemma_norm_pow_inj n (mp' /< 10 +> 1)
   | _ -> ()
 
-let rec lemma_norm_mant_mul' (n: nat) (mp: mant_pow) : Lemma 
-  (requires fst mp <> 0)
-  (ensures norm_pair (fst mp * pow10 n, snd mp) = (fst mp, snd mp + n))
+let rec lemma_norm_neg_inj (mp' : mant_pow') : Lemma
+  (requires True)
+  (ensures norm_pair (mp' *< (-1)) = (norm_pair mp') *< (-1))
+  (decreases abs (fst mp'))
+  =
+  match fst mp', fst mp' % 10 with
+  | 0, _ -> ()
+  | _, 0 -> lemma_norm_neg_inj (mp' /< 10 +> 1)
+  | _, _ -> ()
+
+let lemma_norm_mul10_inj (mp': mant_pow') : Lemma
+  (requires fst mp' <> 0)
+  (ensures norm_pair (mp' *< 10) = (norm_pair mp') +> 1)
+  =
+  assert (norm_pair (mp' *< 10 +> (-1)) = norm_pair mp');
+  lemma_norm_pow_inj 1 (mp' *< 10 +> (-1))
+
+
+
+let rec lemma_norm_pow10_inj' (n: nat) (mp': mant_pow') : Lemma 
+  (requires fst mp' <> 0)
+  (ensures norm_pair (mp' *< pow10 n) = (norm_pair mp') +> n)
   =
   match n with
   | 0 -> ()
   | _ ->
-    lemma_norm_mant_mul' (n - 1) mp;
-    let mant', pow' = fst mp * pow10 (n - 1), snd mp + n - 1 in
-    assert (norm_pair (mant', snd mp) = (fst mp, pow'));
-    lemma_norm_pow_add 1 (mant', snd mp) (mant', snd mp + 1);
-    assert (norm_pair (mant', snd mp + 1) = (fst mp, pow' + 1));
-    assert (norm_pair (mant' * 10, snd mp) = norm_pair (mant', snd mp + 1));
-    assert (norm_pair (mant' * 10, snd mp) = (fst mp, pow' + 1))
+    lemma_norm_pow10_inj' (n - 1) mp';
+    assert (norm_pair (mp' *< pow10 (n - 1)) = (norm_pair mp') +> (n - 1));
+    lemma_norm_mul10_inj (mp' *< pow10 (n - 1));
+    lemma_mant_mul mp' (pow10 (n - 1)) 10;
+    assert (norm_pair (mp' *< pow10 (n - 1) *< 10) = norm_pair (mp' *< pow10 (n - 1)) +> 1);
+    assert (norm_pair (mp' *< pow10 n) = norm_pair mp' +> n)
 
-let lemma_norm_mant_mul (n: nat) (mant: int) (pow: int) : Lemma
+let lemma_norm_pow10_inj (n: nat) (mant: int) (pow: int) : Lemma
   (requires mant % 10 <> 0)
   (ensures norm_pair (mant * pow10 n, pow) = (mant, pow + n))
   [SMTPat (norm_pair (mant * pow10 n, pow))]
-  = lemma_norm_mant_mul' n (mant, pow)
+  = lemma_norm_pow10_inj' n (mant, pow)
 
 val to_pair (x: float) : mant_pow
 val of_pair (mant_power: mant_pow) : float
@@ -89,19 +127,20 @@ val add (a b: float) : Pure float
     let b' = (mantissa b) * pow10 (pow_b - pow_min) in
     to_pair c = norm_pair (a' + b', pow_min))
 
+val neg (a: float) : Pure float
+  (requires True)
+  (ensures fun b -> mantissa a = -(mantissa b) /\ power a = power b)
+
 val sub (a b: float) : Pure float
   (requires True)
   (ensures fun c -> 
-    let mant_a, pow_a = to_pair a in
+    (let mant_a, pow_a = to_pair a in
     let mant_b, pow_b = to_pair b in
     let pow_min = min pow_a pow_b in
     let a' = mant_a * pow10 (pow_a - pow_min) in
     let b' = mant_b * pow10 (pow_b - pow_min) in
     to_pair c = norm_pair (a' - b', pow_min))
-
-val neg (a: float) : Pure float
-  (requires True)
-  (ensures fun b -> mantissa a = -(mantissa b) /\ power a = power b)
+    /\ (c = a `add` (neg b)))
 
 val mul (a b: float) : Pure float
   (requires True)
@@ -115,10 +154,11 @@ val inv (a: not_zero) : Pure not_zero
   (requires True)
   (ensures fun b -> b = one `div` a)
 
-val gt (a b: float) : Pure bool (requires True) (ensures fun c -> c <==> mantissa (a `sub` b) > 0)
-val lt (a b: float) : Pure bool (requires True) (ensures fun c -> c <==> mantissa (a `sub` b) < 0)
-val gte (a b: float) : Pure bool (requires True) (ensures fun c -> c <==> mantissa (a `sub` b) >= 0)
-val lte (a b: float) : Pure bool (requires True) (ensures fun c -> c <==> mantissa (a `sub` b) <= 0)
+val eq (a b: float)  : Pure bool (requires True) (ensures fun c -> c = (mantissa (a `sub` b) = 0) /\ c = (a = b))
+val gt (a b: float)  : Pure bool (requires True) (ensures fun c -> c = (mantissa (a `sub` b) > 0))
+val lt (a b: float)  : Pure bool (requires True) (ensures fun c -> c = (mantissa (a `sub` b) < 0))
+val gte (a b: float) : Pure bool (requires True) (ensures fun c -> c = (mantissa (a `sub` b) >= 0))
+val lte (a b: float) : Pure bool (requires True) (ensures fun c -> c = (mantissa (a `sub` b) <= 0))
 
 val abs (a: float) : Pure float
   (requires True)
@@ -130,54 +170,112 @@ unfold let ( ~. ) a   = neg a
 unfold let ( *. ) a b = mul a b
 unfold let ( /. ) a b = div a b
 
+unfold let (=.) a b = eq a b
 unfold let (>.) a b = gt a b
 unfold let (<.) a b = lt a b
 unfold let (>=.) a b = gte a b
 unfold let (<=.) a b = lte a b
 
+let lemma_gt_zero a b  : Lemma (a  >. b <==> a -. b  >. zero) = ()
+let lemma_lt_zero a b  : Lemma (a  <. b <==> a -. b  <. zero) = ()
+let lemma_gte_zero a b : Lemma (a >=. b <==> a -. b >=. zero) = ()
+let lemma_lte_zero a b : Lemma (a <=. b <==> a -. b <=. zero) = ()
+
+let lemma_gt_lt a b : Lemma (a <. b <==> b >. a) = ()
+let lemma_gte_lte a b : Lemma (a <=. b <==> b >=. a) = ()
+
 let lemma_commut_add a b : Lemma (a +. b = b +. a) = ()
 let lemma_commut_mul a b : Lemma (a *. b = b *. a) = ()
 
-let lemma_add_zero (a: float) : Lemma (a `add` zero = a) = ()
+let lemma_add_zero a : Lemma (a +. zero = a) = ()
 let lemma_mul_one  a : Lemma (a *. one  = a) = ()
 let lemma_mul_zero a : Lemma (a *. zero = zero) = ()
 let lemma_div_one  a : Lemma (a /. one = a) = ()
 
-let test () = assert (zero = of_pair (0, 0))
+let lemma_sub_neg (a: float) : Lemma (~.a = zero -. a) = ()
+let lemma_mul_neg_left (a b: float) : Lemma ((~.a) *. b = ~.(a *. b)) [SMTPat ((~.a) *. b)] =
+  let mant_a, pow_a = to_pair a in
+  let mant_b, pow_b = to_pair b in
+  lemma_norm_neg_inj (mant_a * mant_b, pow_a + pow_b);
+  Lemmas.neg_mul_left mant_a mant_b;
+  assert (norm_pair ((-mant_a) * mant_b, pow_a + pow_b) = norm_pair (-(mant_a * mant_b), pow_a + pow_b));
+  assert (norm_pair (-(mant_a * mant_b), pow_a + pow_b) = norm_pair (mant_a * mant_b, pow_a + pow_b) *< (-1))
+let lemma_mul_neg_right (a b: float) : Lemma (a *. (~.b) = ~.(a *. b)) [SMTPat (a *. (~.b))] =
+  lemma_commut_mul a (~.b)
 
-let lemma_sub_neg (a: float) : Lemma (~.a = zero -. a) =
-  match a = zero with
-  | true -> ()
-  | _ -> 
-    let mant_z, pow_z = to_pair zero in
-    let mant_a, pow_a = to_pair a in
-    let pow_min = min pow_a pow_z in
-    let z' = mant_z * pow10 (pow_z - pow_min) in
-    let a' = mant_a * pow10 (pow_a - pow_min) in
-    match pow_min with
-    | 0 ->
-      assert (z' - a' = - mant_a * pow10 pow_a);
-      lemma_norm_mant_mul pow_a (-mant_a) pow_min
-    | _ -> ()
+let lemma_gt_neg  (a: float) : Lemma (a >.  zero <==> ~.a <. zero) = ()
+let lemma_gte_neg (a: float) : Lemma (a >=. zero <==> ~.a <=. zero) = ()
+let lemma_lt_neg  (a: float) : Lemma (a <.  zero <==> ~.a >. zero) = ()
+let lemma_lte_neg (a: float) : Lemma (a <=. zero <==> ~.a >=. zero) = ()
   
+let lemma_additive_add_left a b c : Lemma (a +. b +. c = (a +. b) +. c) = ()
+let lemma_additive_add_right a b c : Lemma (a +. b +. c = a +. (b +. c)) [SMTPat (a +. b +. c)] = assume (a +. b +. c = a +. (b +. c))
+let lemma_additive_mul_left a b c : Lemma (a *. b *. c = (a *. b) *. c) = ()
+let lemma_additive_mul_right a b c : Lemma (a *. b *. c = a *. (b *. c)) [SMTPat (a *. b *. c)] = assume (a *. b *. c = a *. (b *. c))
+let lemma_distrib_add a b c : Lemma (a *. (b +. c) = a *. b +. a *. c) [SMTPat (a *. (b +. c))] = assume (a *. (b +. c) = a *. b +. a *. c)
+let lemma_distrib_sub a b c : Lemma (a *. (b -. c) = a *. b -. a *. c) [SMTPat (a *. (b -. c))] = ()
+
 let lemma_neg_neg a : Lemma (~.(~.a) = a) = ()
 let lemma_add_neg a : Lemma (a -. a = zero) = ()
 let lemma_sub_add a b : Lemma (a -. b = a +. ~.b) = ()
+
+let lemma_neg_mul a : Lemma (~.a = (~.one) *. a) = ()
+let lemma_distrib_neg a b : Lemma (~.a +. ~.b = ~.(a +. b)) =
+  lemma_neg_mul (a +. b);
+  assert (~.(a +. b) = ~.one *. (a +. b));
+  lemma_distrib_add (~.one) a b;
+  lemma_neg_mul a;
+  lemma_neg_mul b;
+  assert (~.(a +. b) = ~.a +. ~.b)
+let lemma_neg_sub a b : Lemma (a -. b = ~.(b -. a)) =
+  lemma_sub_add b a;
+  lemma_distrib_neg b (~.a);
+  assert (~.(b -. a) = ~.b +. ~.(~.a));
+  lemma_neg_neg a;
+  lemma_commut_add (~.b) a;
+  lemma_sub_add a b
+
+// стоит переписать через обобщённую функцию бинарных отношений
+let lemma_gt_additive a b c : Lemma (requires a >. b) (ensures a +. c >. b +. c) =
+  lemma_gt_zero a b;
+  assert (a -. b >. zero);
+  lemma_add_zero a;
+  lemma_commut_add a zero;
+  assert (a -. b = zero +. a -. b);
+  lemma_add_neg c;
+  assert (a -. b = (c +. ~.c +. a) +. ~.b);
+  lemma_additive_add_right c (~.c) a;
+  lemma_commut_add (~.c) a;
+  lemma_additive_add_right c a (~.c);
+  assert (c +. ~.c +. a = c +. a +. ~.c);
+  lemma_commut_add c a;
+  assert (a -. b = a +. c +. ~.c +. ~.b);
+  lemma_distrib_add (a +. c) (~.c) (~.b);
+  lemma_distrib_neg c b;
+  lemma_sub_add (a +. c) (c +. b);
+  lemma_commut_add c b;
+  assert (a -. b = (a +. c) -. (b +. c));
+  lemma_gt_zero (a +. c) (b +. c)
+let lemma_lt_additive a b c : Lemma (requires a <. b) (ensures a +. c <. b +. c) = lemma_gt_additive b a c
+
+let lemma_gt_add a b c : Lemma (requires a >. c /\ b >. c) (ensures a +. b >. c) = ()
+
+let lemma_commut_gt a b c : Lemma (requires a >. b /\ b >. c) (ensures a >. c) =
+  lemma_gt_zero a b;
+  assert (a -. b >. zero);
+  
+  assume (a >. c);
+  ()
+
 // let lemma_div_inv a : Lemma (a /. a = one) = ()
 // let lemma_inv_inv a : Lemma (inv (inv a) = a) = ()
 
-let lemma_additive_add_left a b c : Lemma (a +. b +. c = (a +. b) +. c) = ()
-let lemma_additive_add_right a b c : Lemma (a +. b +. c = a +. (b +. c)) [SMTPat (a +. b +. c)] =
-  assume (a +. b +. c = a +. (b +. c))
-let lemma_additive_sub_right a b c : Lemma (a +. b -. c = a +. (b -. c)) [SMTPat (a +. b -. c)] =
-  assume (a +. b -. c = a +. (b -. c))
-let lemma_additive_mul_left a b c : Lemma (a *. b *. c = (a *. b) *. c) = ()
-let lemma_additive_mul_right a b c : Lemma (a *. b *. c = a *. (b *. c)) [SMTPat (a *. b *. c)] = 
-  assume (a *. b *. c = a *. (b *. c))
+// let lemma_add_perenos a b c : Lemma (requires a +. b = c) (ensures a = c -. b) =
+//   assert (a +. b -. b = c -. b);
+//   lemma_sub_add (a +. b) b
 
-let lemma_add_perenos a b c : Lemma (requires a +. b = c) (ensures a = c -. b) =
-  assert (a +. b -. b = c -. b);
-  lemma_additive_sub_right a b b
-
-let lemma_distrib_add a b c : Lemma (a *. (b +. c) = a *. b +. a *. c) =
-  assume (a *. (b +. c) = a *. b +. a *. c)
+let lemma_sqr_eq (a b: float) : Lemma
+  (requires a *. a =. b *. b)
+  (ensures (a =. b) \/ (a =. ~.b))
+  =
+  assume ((a = b) \/ (a = ~.b))
